Lean/Egg/Tactic/Config/Modifier.lean
@@ -11,6 +11,7 @@ structure Modifier where
   eraseForallDomains  : Option Bool            := none
   betaReduceRws       : Option Bool            := none
   etaReduceRws        : Option Bool            := none
+  natReduceRws        : Option Bool            := none
   genTcProjRws        : Option Bool            := none
   genTcSpecRws        : Option Bool            := none
   genNatLitRws        : Option Bool            := none
@@ -30,6 +31,7 @@ def modify (cfg : Config) (mod : Modifier) : Config where
   eraseForallDomains  := mod.eraseForallDomains.getD cfg.eraseForallDomains
   betaReduceRws       := mod.betaReduceRws.getD cfg.betaReduceRws
   etaReduceRws        := mod.etaReduceRws.getD cfg.etaReduceRws
+  natReduceRws        := mod.natReduceRws.getD cfg.natReduceRws
   genTcProjRws        := mod.genTcProjRws.getD cfg.genTcProjRws
   genTcSpecRws        := mod.genTcSpecRws.getD cfg.genTcSpecRws
   genNatLitRws        := mod.genNatLitRws.getD cfg.genNatLitRws
