README.md
@@ -4,8 +4,8 @@ This repository contains a (work-in-progress) _equality saturation_ tactic for [
 
 ## Setup
 
-This tactic requires you to have the programming language _Rust_ and its package manager _Cargo_ installed. 
-These are easily installed following the [official guide](https://doc.rust-lang.org/cargo/getting-started/installation.html).
+This tactic requires you to have [Rust](https://www.rust-lang.org) and its package manager [Cargo](https://doc.rust-lang.org/cargo/) installed. 
+They are easily installed following the [official guide](https://doc.rust-lang.org/cargo/getting-started/installation.html).
 
 To use `egg` in your Lean project, add the following line to your `lakefile.lean`:
 
@@ -29,7 +29,7 @@ example (a b c : Nat) (h₁ : a = b) (h₂ : b = c) : a = c := by
   egg [h₁, h₂]
 
 open List in
-theorem reverse_append (as bs : List α) : reverse (as ++ bs) = (reverse bs) ++ (reverse as) := by
+example (as bs : List α) : reverse (as ++ bs) = (reverse bs) ++ (reverse as) := by
   induction as generalizing bs with
   | nil          => egg [reverse_nil, append_nil, append]
   | cons a as ih => egg [ih, append_assoc, reverse_cons, append]
@@ -53,17 +53,15 @@ You can help out by providing _guide terms_ with nudge `egg` to try certain path
 ```lean
 -- From Lean/Egg/Tests/Groups.lean
 
-theorem inv_inv [Group G] (a : G) : -(-a) = a := by
-  egg [/- group axioms -/] using -a + a
+example [Group G] (a : G) : a⁻¹⁻¹ = a := by
+  egg [/- group axioms -/] using a⁻¹ * a
 ```
 
 And if you want to prove your goal based on an equivalent hypothesis, you can use the `from` syntax:
 
 ```lean
-variable (and_assoc : ∀ a b c, (a ∧ b) ∧ c ↔ a ∧ (b ∧ c)) (and_idem : ∀ a, a ↔ a ∧ a)
-
 example (h : p ∧ q ∧ r) : r ∧ r ∧ q ∧ p ∧ q ∧ r ∧ p := by
-  egg [And.comm, and_assoc, and_idem] from h
+  egg [and_comm, and_assoc, and_self] from h
 ```
 
 ## Related Work
